compiler_test/ebpf_test/xdp_prog1.c
@@ -1,0 +1,42 @@
+#include <linux/types.h>
+#include <asm/types.h>
+#include <inttypes.h>
+#include <stdint.h>
+//#include <linux/bpf.h>
+//#include <bpf/bpf_helpers.h>
+#include <bpf.h>
+#include <bpf/bpf_helpers.h>
+
+/*enum xdp_action {
+	XDP_ABORTED = 0,
+	XDP_DROP,
+	XDP_PASS,
+	XDP_TX,
+	XDP_REDIRECT,
+};*/
+
+//static long (* const bpf_trace_printk)(const char *fmt, __u32 fmt_size, ...) = (void *) 6;
+
+#undef bpf_printk
+#define bpf_printk(fmt, ...)                           \
+{                                                      \
+        char ____fmt[] = fmt;                           \
+        bpf_trace_printk(____fmt, sizeof(____fmt),      \
+                         ##__VA_ARGS__);                \
+}
+
+#undef SEC
+#define SEC(A) __attribute__ ((section(A),used))
+
+int counter = 0;
+
+SEC("xdp")
+int packet_count(void *ctx) {
+    bpf_printk("%d", counter);
+    counter = counter + 1;
+    return XDP_PASS;
+}
+
+char LICENSE[] SEC("license") = "Dual BSD/GPL";
+
+
