cparser/Parser.vy
@@ -16,7 +16,8 @@
 
 %{
 
-Require Import List.
+From Coq Require Extraction.
+From Coq Require Import List.
 Require Cabs.
 
 %}
@@ -34,7 +35,8 @@ Require Cabs.
 
 %token<Cabs.loc> LPAREN RPAREN LBRACK RBRACK LBRACE RBRACE DOT COMMA
   SEMICOLON ELLIPSIS TYPEDEF EXTERN STATIC RESTRICT AUTO REGISTER INLINE
-  NORETURN CHAR SHORT INT LONG SIGNED UNSIGNED FLOAT DOUBLE CONST VOLATILE VOID
+  NORETURN CHAR SHORT INT LONG SIGNED UNSIGNED FLOAT FLOAT16 DOUBLE
+  CONST VOLATILE VOID
   STRUCT UNION ENUM UNDERSCORE_BOOL PACKED ALIGNAS ATTRIBUTE ASM
 
 %token<Cabs.loc> CASE DEFAULT IF_ ELSE SWITCH WHILE DO FOR GOTO CONTINUE BREAK
@@ -440,6 +442,8 @@ type_specifier:
     { (Cabs.Tlong, loc) }
 | loc = FLOAT
     { (Cabs.Tfloat, loc) }
+| loc = FLOAT16
+    { (Cabs.Tfloat16, loc) }
 | loc = DOUBLE
     { (Cabs.Tdouble, loc) }
 | loc = SIGNED
@@ -635,18 +639,27 @@ direct_declarator:
 | decl = direct_declarator LBRACK quallst = type_qualifier_list
   expr = assignment_expression RBRACK
     { let 'Cabs.Name name typ attr loc := decl in
-      Cabs.Name name (Cabs.ARRAY typ (rev' quallst) (Some (fst expr))) attr loc }
+      Cabs.Name name (Cabs.ARRAY typ (rev' quallst) false (Some (fst expr))) attr loc }
 | decl = direct_declarator LBRACK expr = assignment_expression RBRACK
     { let 'Cabs.Name name typ attr loc := decl in
-      Cabs.Name name (Cabs.ARRAY typ [] (Some (fst expr))) attr loc }
+      Cabs.Name name (Cabs.ARRAY typ [] false (Some (fst expr))) attr loc }
 | decl = direct_declarator LBRACK quallst = type_qualifier_list RBRACK
     { let 'Cabs.Name name typ attr loc := decl in
-      Cabs.Name name (Cabs.ARRAY typ (rev' quallst) None) attr loc }
+      Cabs.Name name (Cabs.ARRAY typ (rev' quallst) false None) attr loc }
 | decl = direct_declarator LBRACK RBRACK
     { let 'Cabs.Name name typ attr loc := decl in
-      Cabs.Name name (Cabs.ARRAY typ [] None) attr loc }
-(*| direct_declarator LBRACK ... STATIC ... RBRACK
-| direct_declarator LBRACK STAR RBRACK*)
+      Cabs.Name name (Cabs.ARRAY typ [] false None) attr loc }
+| decl = direct_declarator LBRACK STATIC quallst = type_qualifier_list
+  expr = assignment_expression RBRACK
+    { let 'Cabs.Name name typ attr loc := decl in
+      Cabs.Name name (Cabs.ARRAY typ (rev' quallst) true (Some (fst expr))) attr loc }
+| decl = direct_declarator LBRACK STATIC expr = assignment_expression RBRACK
+    { let 'Cabs.Name name typ attr loc := decl in
+      Cabs.Name name (Cabs.ARRAY typ [] true (Some (fst expr))) attr loc }
+| decl = direct_declarator LBRACK quallst = type_qualifier_list STATIC
+  expr = assignment_expression RBRACK
+    { let 'Cabs.Name name typ attr loc := decl in
+      Cabs.Name name (Cabs.ARRAY typ (rev' quallst) true (Some (fst expr))) attr loc }
 | decl = direct_declarator LPAREN params = parameter_type_list RPAREN
     { let 'Cabs.Name name typ attr loc := decl in
       Cabs.Name name (Cabs.PROTO typ params) attr loc }
@@ -720,23 +733,35 @@ direct_abstract_declarator:
     { typ }
 | typ = direct_abstract_declarator LBRACK cvspec = type_qualifier_list
   expr = assignment_expression RBRACK
-    { Cabs.ARRAY typ cvspec (Some (fst expr)) }
+    { Cabs.ARRAY typ cvspec false (Some (fst expr)) }
 | LBRACK cvspec = type_qualifier_list expr = assignment_expression RBRACK
-    { Cabs.ARRAY Cabs.JUSTBASE cvspec (Some (fst expr)) }
+    { Cabs.ARRAY Cabs.JUSTBASE cvspec false (Some (fst expr)) }
 | typ = direct_abstract_declarator LBRACK expr = assignment_expression RBRACK
-    { Cabs.ARRAY typ [] (Some (fst expr)) }
+    { Cabs.ARRAY typ [] false (Some (fst expr)) }
 | LBRACK expr = assignment_expression RBRACK
-    { Cabs.ARRAY Cabs.JUSTBASE [] (Some (fst expr)) }
+    { Cabs.ARRAY Cabs.JUSTBASE [] false (Some (fst expr)) }
 | typ = direct_abstract_declarator LBRACK cvspec = type_qualifier_list RBRACK
-    { Cabs.ARRAY typ cvspec None }
+    { Cabs.ARRAY typ cvspec false None }
 | LBRACK cvspec = type_qualifier_list RBRACK
-    { Cabs.ARRAY Cabs.JUSTBASE cvspec None }
+    { Cabs.ARRAY Cabs.JUSTBASE cvspec false None }
 | typ = direct_abstract_declarator LBRACK RBRACK
-    { Cabs.ARRAY typ [] None }
+    { Cabs.ARRAY typ [] false None }
 | LBRACK RBRACK
-    { Cabs.ARRAY Cabs.JUSTBASE [] None }
-(*| direct_abstract_declarator? LBRACK STAR RBRACK*)
-(*| direct_abstract_declarator? LBRACK ... STATIC ... RBRACK*)
+    { Cabs.ARRAY Cabs.JUSTBASE [] false None }
+| typ = direct_abstract_declarator LBRACK STATIC cvspec = type_qualifier_list
+  expr = assignment_expression RBRACK
+    { Cabs.ARRAY typ cvspec true (Some (fst expr)) }
+| LBRACK STATIC cvspec = type_qualifier_list expr = assignment_expression RBRACK
+    { Cabs.ARRAY Cabs.JUSTBASE cvspec true (Some (fst expr)) }
+| typ = direct_abstract_declarator LBRACK STATIC expr = assignment_expression RBRACK
+    { Cabs.ARRAY typ [] true (Some (fst expr)) }
+| LBRACK STATIC expr = assignment_expression RBRACK
+    { Cabs.ARRAY Cabs.JUSTBASE [] true (Some (fst expr)) }
+| typ = direct_abstract_declarator LBRACK cvspec = type_qualifier_list STATIC
+  expr = assignment_expression RBRACK
+    { Cabs.ARRAY typ cvspec true (Some (fst expr)) }
+| LBRACK cvspec = type_qualifier_list STATIC expr = assignment_expression RBRACK
+    { Cabs.ARRAY Cabs.JUSTBASE cvspec true (Some (fst expr)) }
 | typ = direct_abstract_declarator LPAREN params = parameter_type_list RPAREN
     { Cabs.PROTO typ params }
 | LPAREN params = parameter_type_list RPAREN
