backend/CSEdomain.v
@@ -14,8 +14,9 @@
     subexpression elimination. *)
 
 Require Import Coqlib Maps.
-Require Import AST Integers Values Memory.
+Require Import AST Integers Values Memory Builtins Globalenvs Events.
 Require Import Op Registers RTL.
+Require Import ValueDomain.
 
 (** Value numbers are represented by positive integers.  Equations are
   of the form [valnum = rhs] or [valnum >= rhs], where the right-hand
@@ -27,7 +28,8 @@ Definition valnum := positive.
 
 Inductive rhs : Type :=
   | Op: operation -> list valnum -> rhs
-  | Load: memory_chunk -> addressing -> list valnum -> rhs.
+  | Load: memory_chunk -> addressing -> list valnum -> aptr -> rhs
+  | Builtin: builtin_function -> list (builtin_arg valnum) -> rhs.
 
 Inductive equation : Type :=
   | Eq (v: valnum) (strict: bool) (r: rhs).
@@ -36,12 +38,39 @@ Definition eq_valnum: forall (x y: valnum), {x=y}+{x<>y} := peq.
 
 Definition eq_list_valnum: forall (x y: list valnum), {x=y}+{x<>y} := list_eq_dec peq.
 
-Definition eq_rhs (x y: rhs) : {x=y}+{x<>y}.
-Proof.
-  generalize chunk_eq eq_operation eq_addressing eq_valnum eq_list_valnum.
-  decide equality.
-Defined.
+(** Equality of [rhs] up to differences in regions attached to [Load] rhs. *)
 
+Inductive rhs_compat: rhs -> rhs -> Prop :=
+  | rhs_compat_op: forall op vl,
+      rhs_compat (Op op vl) (Op op vl)
+  | rhs_compat_load: forall chunk addr vl p1 p2,
+      rhs_compat (Load chunk addr vl p1) (Load chunk addr vl p2)
+  | rhs_compat_builtin: forall bf args,
+      rhs_compat (Builtin bf args) (Builtin bf args).
+
+Lemma rhs_compat_sym: forall rh1 rh2,
+  rhs_compat rh1 rh2 -> rhs_compat rh2 rh1.
+Proof.
+  destruct 1; constructor; auto.
+Qed.
+
+Definition compat_rhs (r1 r2: rhs) : bool :=
+  match r1, r2 with
+  | Op op1 vl1, Op op2 vl2 => eq_operation op1 op2 && eq_list_valnum vl1 vl2
+  | Load chunk1 addr1 vl1 p1, Load chunk2 addr2 vl2 p2 =>
+      chunk_eq chunk1 chunk2 && eq_addressing addr1 addr2 && eq_list_valnum vl1 vl2
+  | Builtin bf1 args1, Builtin bf2 args2 =>
+      eq_builtin_function bf1 bf2 && list_eq_dec (eq_builtin_arg eq_valnum) args1 args2
+  | _, _ => false
+  end.
+
+Lemma compat_rhs_sound: forall r1 r2,
+  compat_rhs r1 r2 = true -> rhs_compat r1 r2.
+Proof.
+  unfold compat_rhs; intros; destruct r1, r2; try discriminate;
+  InvBooleans; subst; constructor.
+Qed.
+  
 (** A value numbering is a collection of equations between value numbers
   plus a partial map from registers to value numbers.  Additionally,
   we maintain the next unused value number, so as to easily generate
@@ -69,11 +98,12 @@ Definition empty_numbering :=
 Definition valnums_rhs (r: rhs): list valnum :=
   match r with
   | Op op vl => vl
-  | Load chunk addr vl => vl
+  | Load chunk addr vl ap => vl
+  | Builtin bf args => params_of_builtin_args args
   end.
 
 Definition wf_rhs (next: valnum) (r: rhs) : Prop :=
-forall v, In v (valnums_rhs r) -> Plt v next.
+  forall v, In v (valnums_rhs r) -> Plt v next.
 
 Definition wf_equation (next: valnum) (e: equation) : Prop :=
   match e with Eq l str r => Plt l next /\ wf_rhs next r end.
@@ -101,18 +131,47 @@ Inductive rhs_eval_to (valu: valuation) (ge: genv) (sp: val) (m: mem):
   | op_eval_to: forall op vl v,
       eval_operation ge sp op (map valu vl) m = Some v ->
       rhs_eval_to valu ge sp m (Op op vl) v
-  | load_eval_to: forall chunk addr vl a v,
+  | load_eval_to: forall chunk addr vl a v p,
       eval_addressing ge sp addr (map valu vl) = Some a ->
       Mem.loadv chunk m a = Some v ->
-      rhs_eval_to valu ge sp m (Load chunk addr vl) v.
+      rhs_eval_to valu ge sp m (Load chunk addr vl p) v
+  | builtin_eval_to: forall bf args vargs v,
+      eval_builtin_args ge valu sp m args vargs ->
+      builtin_function_sem bf vargs = Some v ->
+      rhs_eval_to valu ge sp m (Builtin bf args) v.
+
+Lemma rhs_eval_to_compat: forall valu ge sp m rh v rh',
+  rhs_eval_to valu ge sp m rh v ->
+  rhs_compat rh rh' ->
+  rhs_eval_to valu ge sp m rh' v.
+Proof.
+  intros. inv H; inv H0; econstructor; eauto.
+Qed.
+
+(** A [Load] equation carries a region (abstract pointer) [p],
+    characterizing which part of memory is being read.
+    The following predicate makes sure the actual address
+    belongs to the given region. *)
+
+Inductive rhs_valid (valu: valuation) (ge: genv): val -> rhs -> Prop :=
+  | op_valid: forall sp op vl,
+      rhs_valid valu ge sp (Op op vl)
+  | load_valid: forall sp chunk addr vl p b ofs bc,
+      eval_addressing ge (Vptr sp Ptrofs.zero) addr (map valu vl) = Some (Vptr b ofs) ->
+      pmatch bc b ofs p -> genv_match bc ge -> bc sp = BCstack ->
+      rhs_valid valu ge (Vptr sp Ptrofs.zero) (Load chunk addr vl p)
+  | builtin_valid: forall sp bf args,
+      rhs_valid valu ge sp (Builtin bf args).
 
 Inductive equation_holds (valu: valuation) (ge: genv) (sp: val) (m: mem):
                                                       equation -> Prop :=
   | eq_holds_strict: forall l r,
       rhs_eval_to valu ge sp m r (valu l) ->
+      rhs_valid valu ge sp r ->
       equation_holds valu ge sp m (Eq l true r)
   | eq_holds_lessdef: forall l r v,
       rhs_eval_to valu ge sp m r v -> Val.lessdef v (valu l) ->
+      rhs_valid valu ge sp r ->
       equation_holds valu ge sp m (Eq l false r).
 
 Record numbering_holds (valu: valuation) (ge: genv) (sp: val)
