arm/CombineOpproof.v
@@ -13,15 +13,9 @@
 (** Recognition of combined operations, addressing modes and conditions
   during the [CSE] phase. *)
 
-Require Import FunInd.
-Require Import Coqlib.
-Require Import AST.
-Require Import Integers.
-Require Import Values.
-Require Import Memory.
-Require Import Op.
-Require Import Registers.
-Require Import RTL.
+From Coq Require Import FunInd.
+Require Import Coqlib AST Integers Values Memory.
+Require Import Op Registers RTL.
 Require Import CSEdomain.
 Require Import CombineOp.
 
@@ -56,6 +50,9 @@ Proof.
   (* of cmp *)
   UseGetSound. rewrite <- H.
   destruct (eval_condition cond (map valu args) m); simpl; auto. destruct b; auto.
+  (* of xorimm *)
+  UseGetSound. rewrite <- H.
+  destruct v; simpl; auto. rewrite Int.xor_is_zero; auto.
 Qed.
 
 Lemma combine_compimm_eq_0_sound:
@@ -69,6 +66,9 @@ Proof.
   UseGetSound. rewrite <- H.
   rewrite eval_negate_condition.
   destruct (eval_condition c (map valu args) m); simpl; auto. destruct b; auto.
+  (* of xorimm *)
+  UseGetSound. rewrite <- H.
+  destruct v; simpl; auto. rewrite Int.xor_is_zero; auto.
 Qed.
 
 Lemma combine_compimm_eq_1_sound:
