backend/RTLtyping.v
@@ -118,14 +118,14 @@ Inductive wt_instr : instruction -> Prop :=
   | wt_Icall:
       forall sig ros args res s,
       match ros with inl r => env r = Tptr | inr s => True end ->
-      map env args = sig.(sig_args) ->
+      map env args = proj_sig_args sig ->
       env res = proj_sig_res sig ->
       valid_successor s ->
       wt_instr (Icall sig ros args res s)
   | wt_Itailcall:
       forall sig ros args,
       match ros with inl r => env r = Tptr | inr s => True end ->
-      map env args = sig.(sig_args) ->
+      map env args = proj_sig_args sig ->
       sig.(sig_res) = funct.(fn_sig).(sig_res) ->
       tailcall_possible sig ->
       wt_instr (Itailcall sig ros args)
@@ -133,7 +133,7 @@ Inductive wt_instr : instruction -> Prop :=
       forall ef args res s,
       match ef with
       | EF_annot _ _ _ | EF_debug _ _ _ => True
-      | _ => map type_of_builtin_arg args = (ef_sig ef).(sig_args)
+      | _ => map type_of_builtin_arg args = proj_sig_args (ef_sig ef)
       end ->
       type_of_builtin_res res = proj_sig_res (ef_sig ef) ->
       valid_successor s ->
@@ -151,11 +151,11 @@ Inductive wt_instr : instruction -> Prop :=
       list_length_z tbl * 4 <= Int.max_unsigned ->
       wt_instr (Ijumptable arg tbl)
   | wt_Ireturn_none:
-      funct.(fn_sig).(sig_res) = Tvoid ->
+      funct.(fn_sig).(sig_res) = Xvoid ->
       wt_instr (Ireturn None)
   | wt_Ireturn_some:
       forall arg ty,
-      funct.(fn_sig).(sig_res) <> Tvoid ->
+      funct.(fn_sig).(sig_res) <> Xvoid ->
       env arg = proj_sig_res funct.(fn_sig) ->
       env arg = ty ->
       wt_instr (Ireturn (Some arg)).
@@ -170,7 +170,7 @@ End WT_INSTR.
 Record wt_function (f: function) (env: regenv): Prop :=
   mk_wt_function {
     wt_params:
-      map env f.(fn_params) = f.(fn_sig).(sig_args);
+      map env f.(fn_params) = proj_sig_args f.(fn_sig);
     wt_norepet:
       list_norepet f.(fn_params);
     wt_instrs:
@@ -294,12 +294,12 @@ Definition type_instr (e: S.typenv) (i: instruction) : res S.typenv :=
   | Icall sig ros args res s =>
       do x <- check_successor s;
       do e1 <- type_ros e ros;
-      do e2 <- S.set_list e1 args sig.(sig_args);
+      do e2 <- S.set_list e1 args (proj_sig_args sig);
       S.set e2 res (proj_sig_res sig)
   | Itailcall sig ros args =>
       do e1 <- type_ros e ros;
-      do e2 <- S.set_list e1 args sig.(sig_args);
-      if rettype_eq sig.(sig_res) f.(fn_sig).(sig_res) then
+      do e2 <- S.set_list e1 args (proj_sig_args sig);
+      if xtype_eq sig.(sig_res) f.(fn_sig).(sig_res) then
         if tailcall_is_possible sig
         then OK e2
         else Error(msg "tailcall not possible")
@@ -310,7 +310,7 @@ Definition type_instr (e: S.typenv) (i: instruction) : res S.typenv :=
       do e1 <-
         match ef with
         | EF_annot _ _ _ | EF_debug _ _ _ => OK e
-        | _ => type_builtin_args e args sig.(sig_args)
+        | _ => type_builtin_args e args (proj_sig_args sig)
         end;
       type_builtin_res e1 res (proj_sig_res sig)
  | Icond cond args s1 s2 =>
@@ -324,7 +324,7 @@ Definition type_instr (e: S.typenv) (i: instruction) : res S.typenv :=
       then OK e1
       else Error(msg "jumptable too big")
   | Ireturn optres =>
-      match optres, rettype_eq f.(fn_sig).(sig_res) Tvoid with
+      match optres, xtype_eq f.(fn_sig).(sig_res) Xvoid with
       | None, left _ => OK e
       | Some r, right _ => S.set e r (proj_sig_res f.(fn_sig))
       | _, _ => Error(msg "bad return")
@@ -352,7 +352,7 @@ Definition check_params_norepet (params: list reg): res unit :=
 
 Definition type_function : res regenv :=
   do e1 <- type_code S.initial;
-  do e2 <- S.set_list e1 f.(fn_params) f.(fn_sig).(sig_args);
+  do e2 <- S.set_list e1 f.(fn_params) (proj_sig_args f.(fn_sig));
   do te <- S.solve e2;
   do x1 <- check_params_norepet f.(fn_params);
   do x2 <- check_successor f.(fn_entrypoint);
@@ -469,7 +469,7 @@ Proof.
   destruct l; try discriminate. destruct l; monadInv EQ0. eauto with ty.
   destruct (type_of_operation o) as [targs tres] eqn:TYOP. monadInv EQ0. eauto with ty.
 - (* tailcall *)
-  destruct (rettype_eq (sig_res s) (sig_res (fn_sig f))); try discriminate.
+  destruct (xtype_eq (sig_res s) (sig_res (fn_sig f))); try discriminate.
   destruct (tailcall_is_possible s) eqn:TCIP; inv EQ2.
   eauto with ty.
 - (* builtin *)
@@ -479,7 +479,7 @@ Proof.
   eauto with ty.
 - (* return *)
   simpl in H.
-  destruct o as [r|] eqn: RET; destruct (rettype_eq (sig_res (fn_sig f)) Tvoid); try discriminate.
+  destruct o as [r|] eqn: RET; destruct (xtype_eq (sig_res (fn_sig f)) Xvoid); try discriminate.
   eauto with ty.
   inv H; auto with ty.
 Qed.
@@ -521,7 +521,7 @@ Proof.
   eapply S.set_sound; eauto with ty.
   eauto with ty.
 - (* tailcall *)
-  destruct (rettype_eq (sig_res s) (sig_res (fn_sig f))); try discriminate.
+  destruct (xtype_eq (sig_res s) (sig_res (fn_sig f))); try discriminate.
   destruct (tailcall_is_possible s) eqn:TCIP; inv EQ2.
   constructor.
   eapply type_ros_sound; eauto with ty.
@@ -546,7 +546,7 @@ Proof.
   auto.
 - (* return *)
   simpl in H.
-  destruct o as [r|] eqn: RET; destruct (rettype_eq (sig_res (fn_sig f)) Tvoid); try discriminate.
+  destruct o as [r|] eqn: RET; destruct (xtype_eq (sig_res (fn_sig f)) Xvoid); try discriminate.
   econstructor. auto. eapply S.set_sound; eauto with ty. eauto.
   inv H. constructor. auto.
 Qed.
@@ -760,7 +760,7 @@ Proof.
   intros. destruct H.
   destruct (type_code_complete te S.initial) as (e1 & A & B).
   auto. apply S.satisf_initial.
-  destruct (S.set_list_complete te f.(fn_params) f.(fn_sig).(sig_args) e1) as (e2 & C & D); auto.
+  destruct (S.set_list_complete te f.(fn_params) (proj_sig_args f.(fn_sig)) e1) as (e2 & C & D); auto.
   destruct (S.solve_complete te e2) as (te' & E); auto.
   exists te'; unfold type_function.
   rewrite A; simpl. rewrite C; simpl. rewrite E; simpl.
@@ -875,7 +875,7 @@ Qed.
 
 Inductive wt_stackframes: list stackframe -> signature -> Prop :=
   | wt_stackframes_nil: forall sg,
-      sg.(sig_res) = Tint ->
+      sg.(sig_res) = Xint ->
       wt_stackframes nil sg
   | wt_stackframes_cons:
       forall s res f sp pc rs env sg,
@@ -896,7 +896,7 @@ Inductive wt_state: state -> Prop :=
       forall s f args m,
       wt_stackframes s (funsig f) ->
       wt_fundef f ->
-      Val.has_type_list args (sig_args (funsig f)) ->
+      Val.has_type_list args (proj_sig_args (funsig f)) ->
       wt_state (Callstate s f args m)
   | wt_state_return:
       forall s v m sg,
@@ -969,9 +969,9 @@ Proof.
   econstructor; eauto.
   inv WTI; simpl. auto. rewrite <- H3. auto.
   (* internal function *)
-  simpl in *. inv H5.
+  simpl in *. inv H6.
   econstructor; eauto.
-  inv H1. apply wt_init_regs; auto. rewrite wt_params0. auto.
+  inv H2. apply wt_init_regs; auto. rewrite wt_params0. auto.
   (* external function *)
   econstructor; eauto.
   eapply external_call_well_typed; eauto.
